Properties.v
@@ -33,7 +33,7 @@ Ltac solve_q_subtype_wrong :=
   end.
 
 Local Ltac qtypable_contradiction H :=
-  exfalso; unfold qualifier_typable_context, vpa_mutabilty_rs in H; cbn in H; contradiction H.
+  exfalso; unfold qualifier_typable_context, vpa_mutability_rs in H; cbn in H; contradiction H.
 
 Ltac solve_qualifier_typable_wrong_concrete :=
   lazymatch goal with
@@ -66,20 +66,20 @@ Ltac solve_qualifier_typable_wrong_concrete :=
 
 Ltac solve_qualifier_typable_correct_concrete :=
   lazymatch goal with
-  | |- qualifier_typable_context Imm_r Imm Mut_r  => unfold qualifier_typable_context, vpa_mutabilty_rs; cbn; exact I
-  | |- qualifier_typable_context Imm_r RO Mut_r   => unfold qualifier_typable_context, vpa_mutabilty_rs; cbn; exact I
-  | |- qualifier_typable_context Imm_r Lost Mut_r => unfold qualifier_typable_context, vpa_mutabilty_rs; cbn; exact I
-  | |- qualifier_typable_context Imm_r RO Imm_r   => unfold qualifier_typable_context, vpa_mutabilty_rs; cbn; exact I
-  | |- qualifier_typable_context Imm_r Imm Imm_r  => unfold qualifier_typable_context, vpa_mutabilty_rs; cbn; exact I
-  | |- qualifier_typable_context Imm_r Lost Imm_r => unfold qualifier_typable_context, vpa_mutabilty_rs; cbn; exact I
-  | |- qualifier_typable_context Imm_r RDM Imm_r  => unfold qualifier_typable_context, vpa_mutabilty_rs; cbn; exact I
-  | |- qualifier_typable_context Mut_r Mut Mut_r  => unfold qualifier_typable_context, vpa_mutabilty_rs; cbn; exact I
-  | |- qualifier_typable_context Mut_r RO Mut_r   => unfold qualifier_typable_context, vpa_mutabilty_rs; cbn; exact I
-  | |- qualifier_typable_context Mut_r Lost Mut_r => unfold qualifier_typable_context, vpa_mutabilty_rs; cbn; exact I
-  | |- qualifier_typable_context Mut_r RDM Mut_r  => unfold qualifier_typable_context, vpa_mutabilty_rs; cbn; exact I
-  | |- qualifier_typable_context Mut_r RO Imm_r   => unfold qualifier_typable_context, vpa_mutabilty_rs; cbn; exact I
-  | |- qualifier_typable_context Mut_r Mut Imm_r  => unfold qualifier_typable_context, vpa_mutabilty_rs; cbn; exact I
-  | |- qualifier_typable_context Mut_r Lost Imm_r => unfold qualifier_typable_context, vpa_mutabilty_rs; cbn; exact I
+  | |- qualifier_typable_context Imm_r Imm Mut_r  => unfold qualifier_typable_context, vpa_mutability_rs; cbn; exact I
+  | |- qualifier_typable_context Imm_r RO Mut_r   => unfold qualifier_typable_context, vpa_mutability_rs; cbn; exact I
+  | |- qualifier_typable_context Imm_r Lost Mut_r => unfold qualifier_typable_context, vpa_mutability_rs; cbn; exact I
+  | |- qualifier_typable_context Imm_r RO Imm_r   => unfold qualifier_typable_context, vpa_mutability_rs; cbn; exact I
+  | |- qualifier_typable_context Imm_r Imm Imm_r  => unfold qualifier_typable_context, vpa_mutability_rs; cbn; exact I
+  | |- qualifier_typable_context Imm_r Lost Imm_r => unfold qualifier_typable_context, vpa_mutability_rs; cbn; exact I
+  | |- qualifier_typable_context Imm_r RDM Imm_r  => unfold qualifier_typable_context, vpa_mutability_rs; cbn; exact I
+  | |- qualifier_typable_context Mut_r Mut Mut_r  => unfold qualifier_typable_context, vpa_mutability_rs; cbn; exact I
+  | |- qualifier_typable_context Mut_r RO Mut_r   => unfold qualifier_typable_context, vpa_mutability_rs; cbn; exact I
+  | |- qualifier_typable_context Mut_r Lost Mut_r => unfold qualifier_typable_context, vpa_mutability_rs; cbn; exact I
+  | |- qualifier_typable_context Mut_r RDM Mut_r  => unfold qualifier_typable_context, vpa_mutability_rs; cbn; exact I
+  | |- qualifier_typable_context Mut_r RO Imm_r   => unfold qualifier_typable_context, vpa_mutability_rs; cbn; exact I
+  | |- qualifier_typable_context Mut_r Mut Imm_r  => unfold qualifier_typable_context, vpa_mutability_rs; cbn; exact I
+  | |- qualifier_typable_context Mut_r Lost Imm_r => unfold qualifier_typable_context, vpa_mutability_rs; cbn; exact I
   end.
 
 Lemma collect_methods_exists : forall CT C
@@ -761,24 +761,24 @@ Qed.
 
 Lemma sq_vpa_tt_eq_qq_abs_imm :
   forall T1 T2,
-    sqtype (vpa_mutabilty_tt_abs_imm T1 T2)
-    = vpa_mutabilty_qq_abs_imm (sqtype T1) (sqtype T2).
+    sqtype (vpa_mutability_tt_abs_imm T1 T2)
+    = vpa_mutability_qq_abs_imm (sqtype T1) (sqtype T2).
 Proof.
   intros T1 T2.
   destruct T1 as [q1 c1], T2 as [q2 c2].
-  unfold vpa_mutabilty_tt_abs_imm, vpa_mutabilty_qq_abs_imm.
+  unfold vpa_mutability_tt_abs_imm, vpa_mutability_qq_abs_imm.
   simpl.
   destruct q1; destruct q2; reflexivity.
 Qed.
 
 Lemma sq_vpa_tt_eq_qq_safe_ro :
   forall T1 T2,
-    sqtype (vpa_mutabilty_tt_safe_ro T1 T2)
-    = vpa_mutabilty_qq_safe_ro (sqtype T1) (sqtype T2).
+    sqtype (vpa_mutability_tt_safe_ro T1 T2)
+    = vpa_mutability_qq_safe_ro (sqtype T1) (sqtype T2).
 Proof.
   intros T1 T2.
   destruct T1 as [q1 c1], T2 as [q2 c2].
-  unfold vpa_mutabilty_tt_safe_ro, vpa_mutabilty_qq_safe_ro.
+  unfold vpa_mutability_tt_safe_ro, vpa_mutability_qq_safe_ro.
   simpl.
   destruct q1; destruct q2; reflexivity.
 Qed.
@@ -918,7 +918,7 @@ Proof.
   destruct rq as [|]; destruct (sqtype Ty1); destruct (sqtype Ty2);
   simpl in *; auto;
   try (inversion Hsubtype; auto);
-  try unfold vpa_mutabilty_rs in *;
+  try unfold vpa_mutability_rs in *;
   try destruct qcontext;
   try reflexivity;
   try easy.
@@ -1908,7 +1908,7 @@ Proof.
                   unfold qualifier_typable_heap.
                   move Hsub at bottom.
                   move Hqual_typable at bottom.
-                  unfold vpa_mutabilty_rec_fld; unfold vpa_mutabilty_stype_fld_abs_imm in Hsub.
+                  unfold vpa_mutability_rec_fld; unfold vpa_mutability_stype_fld_abs_imm in Hsub.
                   subst rqt_x.
 
                   clear - Hsub Hqual_typable Hxyqualifer.
@@ -1988,9 +1988,9 @@ Proof.
                 rewrite Hobj_lx in Hcorr.
                 destruct Hcorr as [_ Hqualifiertypablex].
                 inversion Hgetobj; subst o.
-                unfold vpa_mutabilty_stype_fld_abs_imm in Hsub.
-                unfold vpa_mutabilty_rec_fld.
-                unfold vpa_mutabilty_rs in Hqual_y.
+                unfold vpa_mutability_stype_fld_abs_imm in Hsub.
+                unfold vpa_mutability_rec_fld.
+                unfold vpa_mutability_rs in Hqual_y.
                 clear - Hqual_y Hsub Hqualifiertypablex.
                 all:
                 destruct (rqtype rqt_y) eqn: Hrqy;
@@ -2406,7 +2406,7 @@ Proof.
                 unfold qualifier_typable_heap.
                 move Hsub at bottom.
                 move Hqual_typable at bottom.
-                unfold vpa_mutabilty_rec_fld; unfold vpa_mutabilty_stype_fld_abs_imm in Hsub.
+                unfold vpa_mutability_rec_fld; unfold vpa_mutability_stype_fld_abs_imm in Hsub.
                 subst rqt_x.
 
                 clear - Hsub Hqual_typable Hxyqualifer.
@@ -2486,9 +2486,9 @@ Proof.
                 rewrite Hobj_lx in Hcorr.
                 destruct Hcorr as [_ Hqualifiertypablex].
                 inversion Hgetobj; subst o.
-                unfold vpa_mutabilty_stype_fld_abs_imm in Hsub.
-                unfold vpa_mutabilty_rec_fld.
-                unfold vpa_mutabilty_rs in Hqual_y.
+                unfold vpa_mutability_stype_fld_abs_imm in Hsub.
+                unfold vpa_mutability_rec_fld.
+                unfold vpa_mutability_rs in Hqual_y.
                 clear - Hqual_y Hsub Hqualifiertypablex.
                 all:
                 destruct (rqtype rqt_y) eqn: Hrqy;
@@ -2904,7 +2904,7 @@ Proof.
                   unfold qualifier_typable_heap.
                   move Hsub at bottom.
                   move Hqual_typable at bottom.
-                  unfold vpa_mutabilty_rec_fld; unfold vpa_mutabilty_stype_fld_abs_imm in Hsub.
+                  unfold vpa_mutability_rec_fld; unfold vpa_mutability_stype_fld_abs_imm in Hsub.
                   subst rqt_x.
 
                   clear - Hsub Hqual_typable Hxyqualifer.
@@ -2984,9 +2984,9 @@ Proof.
                 rewrite Hobj_lx in Hcorr.
                 destruct Hcorr as [_ Hqualifiertypablex].
                 inversion Hgetobj; subst o.
-                unfold vpa_mutabilty_stype_fld_abs_imm in Hsub.
-                unfold vpa_mutabilty_rec_fld.
-                unfold vpa_mutabilty_rs in Hqual_y.
+                unfold vpa_mutability_stype_fld_abs_imm in Hsub.
+                unfold vpa_mutability_rec_fld.
+                unfold vpa_mutability_rs in Hqual_y.
                 clear - Hqual_y Hsub Hqualifiertypablex.
                 all:
                 destruct (rqtype rqt_y) eqn: Hrqy;
@@ -3274,7 +3274,7 @@ Proof.
         ** apply find_class_dom in Hfind.
           split.
           exact Hfind.
-          unfold vpa_mutabilty_runtime_bound_agree.
+          unfold vpa_mutability_runtime_bound_agree.
           assert (Hwf_ctor : wf_constructor CT c consig).
           {
             eapply constructor_lookup_wf; eauto.
@@ -3283,8 +3283,8 @@ Proof.
           destruct Hwf_ctor as [Hctor_bound [Hparamswf [field_defs [Hcollect_H1 [Hdom_eq Hfieldtypematch]]]]].
           rewrite Hbound in Hctor_bound.
           inversion Hctor_bound; subst.
-          unfold vpa_mutabilty_object_creation.
-          unfold vpa_mutabilty_bound in Hqc.
+          unfold vpa_mutability_object_creation.
+          unfold vpa_mutability_bound in Hqc.
           destruct q_c eqn:Hnewq;
           destruct (cqualifier consig) eqn: Hcbound;
           destruct qthisr eqn: Hqthis;
@@ -3498,9 +3498,9 @@ Proof.
             discriminate Hrtype_receiver.
           }
           unfold qualifier_typable_heap.
-          unfold vpa_mutabilty_rec_fld.
-          unfold vpa_mutabilty_constructor_fld in Hfieldtypematch.
-          unfold vpa_mutabilty_object_creation.
+          unfold vpa_mutability_rec_fld.
+          unfold vpa_mutability_constructor_fld in Hfieldtypematch.
+          unfold vpa_mutability_object_creation.
           unfold qc2q in Hresult_sub.
           simpl in Hresult_sub.
           assert (l1 = ι). {
@@ -3515,7 +3515,7 @@ Proof.
             inversion HgetthisRuntimeType; reflexivity.
           }
           subst qthisr.
-	          unfold vpa_mutabilty_bound in Hqc.
+	          unfold vpa_mutability_bound in Hqc.
 	          clear - Hfieldtypematch Hqctype Harg_sub Hqc.
 	          destruct (rqtype rqt) eqn: Hrqtq;
 	          destruct qcontext eqn: Hqthis;
@@ -3628,7 +3628,7 @@ Proof.
       assert (dom h + 1 = S (dom h)) by lia.
       unfold runtime_getObj.
       simpl.
-	      assert (Hlen_extended: dom (h ++ [{| rt_type := {| rqtype := vpa_mutabilty_object_creation
+	      assert (Hlen_extended: dom (h ++ [{| rt_type := {| rqtype := vpa_mutability_object_creation
 qthisr q_c; rctype := c |}; fields_map := vals |}]) = dom h + 1).
       -- rewrite length_app. simpl. lia.
       -- rewrite nth_error_app2.
@@ -3754,11 +3754,11 @@ qthisr q_c; rctype := c |}; fields_map := vals |}]) = dom h + 1).
               }
               subst qthisr.
               unfold qualifier_typable_context in *.
-              unfold vpa_mutabilty_object_creation in *.
-	              unfold vpa_mutabilty_rs in *;
+              unfold vpa_mutability_object_creation in *.
+	              unfold vpa_mutability_rs in *;
 	              unfold qc2q in *;
-	              unfold vpa_mutabilty_tt_abs_imm in *.
-	              unfold vpa_mutabilty_bound in Hqc.
+	              unfold vpa_mutability_tt_abs_imm in *.
+	              unfold vpa_mutability_bound in Hqc.
 	              destruct q_c eqn:Hnewq;
 	              destruct (cqualifier consig) eqn: Hcbound;
 	              destruct qcontext eqn: Hqcontext;
@@ -3798,7 +3798,7 @@ qthisr q_c; rctype := c |}; fields_map := vals |}]) = dom h + 1).
         rewrite Hval.
         unfold wf_r_typable in Hcorr_orig |- *.
         destruct (r_type h loc) as [rqt|] eqn:Hrtype; [|contradiction].
-	          assert (Hrtype_ext : r_type (h ++ [{| rt_type := {| rqtype := vpa_mutabilty_object_creation qthisr
+	          assert (Hrtype_ext : r_type (h ++ [{| rt_type := {| rqtype := vpa_mutability_object_creation qthisr
 q_c; rctype := c |}; fields_map := vals |}]) loc = Some rqt).
           {
             unfold r_type in Hrtype |- *.
@@ -3812,23 +3812,23 @@ q_c; rctype := c |}; fields_map := vals |}]) loc = Some rqt).
           }
 Qed.
 
-Lemma vpa_mutabilty_tt_sctype_abs_imm :
+Lemma vpa_mutability_tt_sctype_abs_imm :
   forall Tthis T : qualified_type,
-    sctype (vpa_mutabilty_tt_abs_imm Tthis T) = sctype T.
+    sctype (vpa_mutability_tt_abs_imm Tthis T) = sctype T.
 Proof.
   intros Tthis [q c].
-  unfold vpa_mutabilty_tt_abs_imm.    
+  unfold vpa_mutability_tt_abs_imm.
   simpl.
   destruct (sqtype Tthis); simpl; try reflexivity.
   all: destruct q; simpl; reflexivity.
 Qed.
 
-Lemma vpa_mutabilty_tt_sctype_safe_ro :
+Lemma vpa_mutability_tt_sctype_safe_ro :
   forall Tthis T : qualified_type,
-    sctype (vpa_mutabilty_tt_safe_ro Tthis T) = sctype T.
+    sctype (vpa_mutability_tt_safe_ro Tthis T) = sctype T.
 Proof.
   intros Tthis [q c].
-  unfold vpa_mutabilty_tt_safe_ro.    
+  unfold vpa_mutability_tt_safe_ro.
   simpl.
   destruct (sqtype Tthis); simpl; try reflexivity.
   all: destruct q; simpl; reflexivity.
