ReadonlyConfinement.v
@@ -403,7 +403,7 @@ Proof.
         rewrite Hmsigeq.
         destruct Hrcv_sub as [Hrcv_sub | Hrcv_sub].
         apply qualified_type_subtype_base_subtype in Hrcv_sub.
-        rewrite (vpa_mutabilty_tt_sctype_safe_ro Ty (mreceiver (msignature mdef0))) in Hrcv_sub.
+        rewrite (vpa_mutability_tt_sctype_safe_ro Ty (mreceiver (msignature mdef0))) in Hrcv_sub.
         eapply base_trans; eauto.
         destruct Hrcv_sub as [HTyqualifier [HReceiverDeclearedQualifier HBaseSubtype]].
         eapply base_trans; eauto.
@@ -465,10 +465,10 @@ Proof.
             unfold qualifier_typable_context.
             unfold qualifier_typable_context in HyQualifierTypablility.
             unfold qualifier_typable_context in Houtter_qualifier_typable.
-            unfold vpa_mutabilty_rs.
-            unfold vpa_mutabilty_rs in HyQualifierTypablility.
-            unfold vpa_mutabilty_rs in Houtter_qualifier_typable.
-            unfold vpa_mutabilty_tt_safe_ro in Hrcv_sub.
+            unfold vpa_mutability_rs.
+            unfold vpa_mutability_rs in HyQualifierTypablility.
+            unfold vpa_mutability_rs in Houtter_qualifier_typable.
+            unfold vpa_mutability_tt_safe_ro in Hrcv_sub.
             rewrite <- Hmsigeq in Hrcv_sub.
 
             destruct qinner eqn:HInnerReceiverMutability;
@@ -537,9 +537,9 @@ Proof.
             unfold qualifier_typable_context.
             unfold qualifier_typable_context in HyQualifierTypablility.
             unfold qualifier_typable_context in Houtter_qualifier_typable.
-            unfold vpa_mutabilty_rs.
-            unfold vpa_mutabilty_rs in HyQualifierTypablility.
-            unfold vpa_mutabilty_rs in Houtter_qualifier_typable.
+            unfold vpa_mutability_rs.
+            unfold vpa_mutability_rs in HyQualifierTypablility.
+            unfold vpa_mutability_rs in Houtter_qualifier_typable.
             rewrite <- Hmsigeq in HReceiverDeclearedQualifier.
 
             destruct qinner eqn:HInnerReceiverMutability;
@@ -656,7 +656,7 @@ Proof.
             rewrite Hmsigeq in Hnth.
             eapply Forall2_nth_error in Harg_sub; eauto.
             apply qualified_type_subtype_base_subtype in Harg_sub.
-            rewrite (vpa_mutabilty_tt_sctype_safe_ro Ty sqt) in Harg_sub.
+            rewrite (vpa_mutability_tt_sctype_safe_ro Ty sqt) in Harg_sub.
             eapply base_trans; eauto.
 
             (* Qualifier Typability *)
@@ -766,7 +766,7 @@ Proof.
         exact Hconfined.
       }
       unfold is_safe_mode in Hty_safe.
-      unfold vpa_mutabilty_tt_safe_ro.
+      unfold vpa_mutability_tt_safe_ro.
       assert (Hy_dom : y < dom sΓ).
       {
         apply static_getType_dom in Hget_y.
@@ -816,7 +816,7 @@ Proof.
       destruct Hrcv_sub as [Hrcv_sub | Hrcv_sub].
       apply qualified_type_subtype_q_subtype in Hrcv_sub.
       rewrite Hmsigeq.
-      unfold vpa_mutabilty_tt_safe_ro in Hrcv_sub.
+      unfold vpa_mutability_tt_safe_ro in Hrcv_sub.
       destruct Hty_safe as [HRd | [HLost| [HRDM | HImm]]].
       + (* Case: sqtype Ty = Rd *)
         rewrite HRd in Hrcv_sub.
@@ -1548,8 +1548,8 @@ Proof.
         rewrite Hmsigeq.
         destruct Hrcv_sub as [Hrcv_sub | Hrcv_sub].
         apply qualified_type_subtype_base_subtype in Hrcv_sub.
-        (* rewrite (vpa_mutabilty_tt_sctype Tthis Ty) in Hmethod_case. *)
-        rewrite (vpa_mutabilty_tt_sctype_safe_ro Ty (mreceiver (msignature mdef0))) in Hrcv_sub.
+        (* rewrite (vpa_mutability_tt_sctype Tthis Ty) in Hmethod_case. *)
+        rewrite (vpa_mutability_tt_sctype_safe_ro Ty (mreceiver (msignature mdef0))) in Hrcv_sub.
         eapply base_trans; eauto.
         destruct Hrcv_sub as [HTyqualifier [HReceiverDeclearedQualifier HBaseSubtype]].
         eapply base_trans; eauto.
@@ -1612,10 +1612,10 @@ Proof.
             unfold qualifier_typable_context.
             unfold qualifier_typable_context in HyQualifierTypablility.
             unfold qualifier_typable_context in Houtter_qualifier_typable.
-            unfold vpa_mutabilty_rs.
-            unfold vpa_mutabilty_rs in HyQualifierTypablility.
-            unfold vpa_mutabilty_rs in Houtter_qualifier_typable.
-            unfold vpa_mutabilty_tt_safe_ro in Hrcv_sub.
+            unfold vpa_mutability_rs.
+            unfold vpa_mutability_rs in HyQualifierTypablility.
+            unfold vpa_mutability_rs in Houtter_qualifier_typable.
+            unfold vpa_mutability_tt_safe_ro in Hrcv_sub.
             rewrite <- Hmsigeq in Hrcv_sub.
 
             destruct qinner eqn:HInnerReceiverMutability;
@@ -1684,9 +1684,9 @@ Proof.
             unfold qualifier_typable_context.
             unfold qualifier_typable_context in HyQualifierTypablility.
             unfold qualifier_typable_context in Houtter_qualifier_typable.
-            unfold vpa_mutabilty_rs.
-            unfold vpa_mutabilty_rs in HyQualifierTypablility.
-            unfold vpa_mutabilty_rs in Houtter_qualifier_typable.
+            unfold vpa_mutability_rs.
+            unfold vpa_mutability_rs in HyQualifierTypablility.
+            unfold vpa_mutability_rs in Houtter_qualifier_typable.
             rewrite <- Hmsigeq in HReceiverDeclearedQualifier.
 
             destruct qinner eqn:HInnerReceiverMutability;
@@ -1802,7 +1802,7 @@ Proof.
             rewrite Hmsigeq in Hnth.
             eapply Forall2_nth_error in Harg_sub; eauto.
             apply qualified_type_subtype_base_subtype in Harg_sub.
-            rewrite (vpa_mutabilty_tt_sctype_safe_ro Ty sqt) in Harg_sub.
+            rewrite (vpa_mutability_tt_sctype_safe_ro Ty sqt) in Harg_sub.
             eapply base_trans; eauto.
 
             (* Qualifier Typability *)
@@ -1913,7 +1913,7 @@ Proof.
         exact Hconfined.
       }
       unfold is_safe_mode in Hty_safe.
-      unfold vpa_mutabilty_tt_safe_ro.
+      unfold vpa_mutability_tt_safe_ro.
       assert (Hy_dom : y < dom sΓ).
       {
         apply static_getType_dom in Hget_y.
@@ -1962,7 +1962,7 @@ Proof.
       destruct Hrcv_sub as [Hrcv_sub | Hrcv_sub].
       clear - Hmsigeq Hty_safe Hrcv_sub.
       rewrite Hmsigeq.
-      unfold vpa_mutabilty_tt_safe_ro in Hrcv_sub.
+      unfold vpa_mutability_tt_safe_ro in Hrcv_sub.
       apply qualified_type_subtype_q_subtype in Hrcv_sub.
       destruct Hty_safe as [HRd | [HLost | [HRDM | HImm]]].
       + (* Case: sqtype Ty = Rd *)
