ReadonlySafety.v
@@ -616,7 +616,7 @@ Theorem readonly_method_call_preserves_arguments :
         rewrite Hmsigeq.
         destruct Hrcv_sub as [Hrcv_sub | Hrcv_sub].
         apply qualified_type_subtype_base_subtype in Hrcv_sub.
-        rewrite (vpa_mutabilty_tt_sctype_safe_ro Ty (mreceiver (msignature mdef1))) in Hrcv_sub.
+        rewrite (vpa_mutability_tt_sctype_safe_ro Ty (mreceiver (msignature mdef1))) in Hrcv_sub.
         eapply base_trans; eauto.
         destruct Hrcv_sub as [HTyqualifier [HReceiverDeclearedQualifier HBaseSubtype]].
         eapply base_trans; eauto.
@@ -678,10 +678,10 @@ Theorem readonly_method_call_preserves_arguments :
             unfold qualifier_typable_context.
             unfold qualifier_typable_context in HyQualifierTypablility.
             unfold qualifier_typable_context in Houtter_qualifier_typable.
-            unfold vpa_mutabilty_rs.
-            unfold vpa_mutabilty_rs in HyQualifierTypablility.
-            unfold vpa_mutabilty_rs in Houtter_qualifier_typable.
-            unfold vpa_mutabilty_tt_safe_ro in Hrcv_sub.
+            unfold vpa_mutability_rs.
+            unfold vpa_mutability_rs in HyQualifierTypablility.
+            unfold vpa_mutability_rs in Houtter_qualifier_typable.
+            unfold vpa_mutability_tt_safe_ro in Hrcv_sub.
             rewrite <- Hmsigeq in Hrcv_sub.
 
             destruct qinner eqn:HInnerReceiverMutability;
@@ -750,9 +750,9 @@ Theorem readonly_method_call_preserves_arguments :
             unfold qualifier_typable_context.
             unfold qualifier_typable_context in HyQualifierTypablility.
             unfold qualifier_typable_context in Houtter_qualifier_typable.
-            unfold vpa_mutabilty_rs.
-            unfold vpa_mutabilty_rs in HyQualifierTypablility.
-            unfold vpa_mutabilty_rs in Houtter_qualifier_typable.
+            unfold vpa_mutability_rs.
+            unfold vpa_mutability_rs in HyQualifierTypablility.
+            unfold vpa_mutability_rs in Houtter_qualifier_typable.
             rewrite <- Hmsigeq in HReceiverDeclearedQualifier.
 
             rewrite HReceiverDeclearedQualifier.
@@ -862,7 +862,7 @@ Theorem readonly_method_call_preserves_arguments :
             rewrite Hmsigeq in Hnth.
             eapply Forall2_nth_error in Harg_sub; eauto.
             apply qualified_type_subtype_base_subtype in Harg_sub.
-            rewrite (vpa_mutabilty_tt_sctype_safe_ro Ty sqt) in Harg_sub.
+            rewrite (vpa_mutability_tt_sctype_safe_ro Ty sqt) in Harg_sub.
             eapply base_trans; eauto.
 
             (* Qualifier Typability *)
@@ -1279,8 +1279,8 @@ Theorem readonly_method_call_preserves_arguments :
         rewrite Hmsigeq.
         destruct Hrcv_sub as [Hrcv_sub | Hrcv_sub].
         apply qualified_type_subtype_base_subtype in Hrcv_sub.
-        (* rewrite (vpa_mutabilty_tt_sctype Tthis Ty) in Hrcv_sub. *)
-        rewrite (vpa_mutabilty_tt_sctype_safe_ro Ty (mreceiver (msignature mdef1))) in Hrcv_sub.
+        (* rewrite (vpa_mutability_tt_sctype Tthis Ty) in Hrcv_sub. *)
+        rewrite (vpa_mutability_tt_sctype_safe_ro Ty (mreceiver (msignature mdef1))) in Hrcv_sub.
         eapply base_trans; eauto.
         destruct Hrcv_sub as [HTyqualifier [HReceiverDeclearedQualifier HBaseSubtype]].
         eapply base_trans; eauto.
@@ -1342,10 +1342,10 @@ Theorem readonly_method_call_preserves_arguments :
             unfold qualifier_typable_context.
             unfold qualifier_typable_context in HyQualifierTypablility.
             unfold qualifier_typable_context in Houtter_qualifier_typable.
-            unfold vpa_mutabilty_rs.
-            unfold vpa_mutabilty_rs in HyQualifierTypablility.
-            unfold vpa_mutabilty_rs in Houtter_qualifier_typable.
-            unfold vpa_mutabilty_tt_safe_ro in Hrcv_sub.
+            unfold vpa_mutability_rs.
+            unfold vpa_mutability_rs in HyQualifierTypablility.
+            unfold vpa_mutability_rs in Houtter_qualifier_typable.
+            unfold vpa_mutability_tt_safe_ro in Hrcv_sub.
             rewrite <- Hmsigeq in Hrcv_sub.
 
             destruct qinner eqn:HInnerReceiverMutability;
@@ -1414,9 +1414,9 @@ Theorem readonly_method_call_preserves_arguments :
             unfold qualifier_typable_context.
             unfold qualifier_typable_context in HyQualifierTypablility.
             unfold qualifier_typable_context in Houtter_qualifier_typable.
-            unfold vpa_mutabilty_rs.
-            unfold vpa_mutabilty_rs in HyQualifierTypablility.
-            unfold vpa_mutabilty_rs in Houtter_qualifier_typable.
+            unfold vpa_mutability_rs.
+            unfold vpa_mutability_rs in HyQualifierTypablility.
+            unfold vpa_mutability_rs in Houtter_qualifier_typable.
             rewrite <- Hmsigeq in HReceiverDeclearedQualifier.
             rewrite HReceiverDeclearedQualifier;
             destruct qinner eqn:HInnerReceiverMutability;
@@ -1527,7 +1527,7 @@ Theorem readonly_method_call_preserves_arguments :
             rewrite Hmsigeq in Hnth.
             eapply Forall2_nth_error in Harg_sub; eauto.
             apply qualified_type_subtype_base_subtype in Harg_sub.
-            rewrite (vpa_mutabilty_tt_sctype_safe_ro Ty sqt) in Harg_sub.
+            rewrite (vpa_mutability_tt_sctype_safe_ro Ty sqt) in Harg_sub.
             eapply base_trans; eauto.
 
             (* Qualifier Typability *)
